disk-betree/PivotBetreeSpec.dfy
@@ -1,6 +1,7 @@
 include "BlockInterface.dfy"  
 include "../lib/sequences.dfy"
 include "../lib/Maps.dfy"
+include "../lib/Sets.dfy"
 include "MapSpec.dfy"
 include "Graph.dfy"
 include "../tla-tree/MissingLibrary.dfy"
